proof/uni_rec/ltac_utils.v
@@ -21,6 +21,23 @@ Ltac inst_cofinites_with x :=
     end
 .
 
+Ltac inst_cofinite_impl_keep H x :=
+  match type of H with
+    | forall x, x `notin` ?L -> _ =>
+      let H_1 := fresh "H" in
+        let Fr := fresh "Fr" in
+          assert (x `notin` L) as Fr by auto;
+          specialize (H x Fr) as H_1; generalize dependent H
+  end.
+
+Ltac inst_cofinites_with_keep x :=
+  repeat
+    match goal with
+      | H : forall x0, x0 `notin` ?L -> _ |- _ =>
+          inst_cofinite_impl_keep H x
+    end;
+  intros.
+
 Ltac inst_cofinites :=
   match goal with
   | x : atom |- _ => inst_cofinites_with x
@@ -88,7 +105,7 @@ Ltac gather_atoms ::=
 
 Ltac solve_wf_twl_sub_false :=
   match goal with
-  | H : (∃ A B : typ, work_sub ?A' ?B' = work_sub A B) → False |- _ => exfalso; eauto
+  | H : (exists A B : typ, work_sub ?A' ?B' = work_sub A B) -> False |- _ => exfalso; eauto
   | _ : _ |- _ => idtac
   end.
 
@@ -168,4 +185,5 @@ Ltac destruct_in :=
     try solve [solve_notin_eq X];
     try solve [solve_notin_eq X']
   end.
+  
                                 
